Ctauto.v
@@ -1,0 +1,3 @@
+Require Export Cdcl.Itauto.
+(** itauto is using the `classic` axiom if available *)
+#[export] Set Itauto Classic.
