test-suite/btauto.v
@@ -1,0 +1,16 @@
+Require Import Cdcl.Itauto.
+
+Open Scope bool_scope.
+
+Require Import Btauto.
+
+Lemma test_neg_involutive b :  negb (negb b) = b.
+Proof.
+  itauto. Qed.
+
+Lemma test_orb a b : (if a || b then negb (negb b && negb a) else negb a && negb b) = true.
+Proof.
+  itauto. Qed.
+
+Lemma test_xorb a : xorb a a = false.
+Proof. itauto. Qed.
