theories/CnfSolver.v
@@ -1,0 +1,2174 @@
+Require Import ZArith.
+Require Import List Bool Btauto.
+Require Import Morphisms.
+
+Ltac inv H := inversion H ; try subst ; clear H.
+
+Inductive sublist {A: Type}: list A -> list A -> Prop :=
+| SUB_NIL : forall l, sublist nil l
+| SUB_CONS : forall l1 l2 a, sublist l1 l2 -> sublist l1 (a::l2)
+| SUB_CONS2: forall l1 l2 a, sublist l1 l2 -> sublist (a::l1) (a::l2).
+
+Lemma sublist_refl : forall {A: Type} (l: list A),
+    sublist l l.
+Proof.
+  induction l.
+  - constructor.
+  - apply SUB_CONS2. auto.
+Qed.
+
+Module Lit.
+
+  Inductive t :=
+  | POS (p:positive)
+  | NEG (p:positive).
+
+  Definition pol (x:t) :=
+    match x with
+    | POS _ => true
+    | NEG _ => false
+    end.
+
+  Definition isPOS (x:t) :=
+    pol x = true.
+
+
+  Definition var (x:t) :=
+    match x with
+    | POS p => p
+    | NEG p => p
+    end.
+
+  Definition neg (x:t) :=
+    match x with
+    | POS x => NEG x
+    | NEG x => POS x
+    end.
+
+
+  Definition beval_lit (env : positive -> bool) (l:t) :=
+    if pol l then env (var l) else
+      negb (env (var l)).
+
+  Definition eval_lit (env: positive -> Prop) (l:t) (X:Prop)  :=
+    if pol l then env (var l) \/ X
+             else env (var l) -> X.
+
+  Lemma beval_lit_neg : forall env l,
+      beval_lit env l = negb (beval_lit env (neg l)).
+  Proof.
+    unfold beval_lit.
+    destruct l; simpl; auto.
+    rewrite negb_involutive. reflexivity.
+  Qed.
+
+  
+  Add Parametric Morphism (env:positive -> Prop) (l:t) : (eval_lit env l) with signature iff ==> iff as eval_lit_morph.
+  Proof.
+    unfold eval_lit.
+    intros.
+    destruct (pol l). tauto.
+    tauto.
+  Qed.
+
+  Definition get_pol (p:positive) (l : Lit.t) : option bool :=
+    if Pos.eqb p (var l) then Some (pol l) else None.
+
+  Definition eq_dec (l1 l2:t) : {l1 = l2} + {l1 <> l2}.
+  Proof.
+    decide equality.
+    apply Pos.eq_dec.
+    apply Pos.eq_dec.
+  Qed.
+
+  Definition make (b:bool) (v:positive) :=
+    if b then POS v else NEG v.
+
+  Lemma var_make : forall b v, var (make b v) = v.
+  Proof.
+    unfold make. destruct b;reflexivity.
+  Qed.
+
+  Lemma decomp : forall l,
+      l = (if pol l then POS (var l) else NEG (var l)).
+  Proof.
+    destruct l; reflexivity.
+  Qed.
+
+  Lemma get_pol_inv : forall p l b,
+      get_pol p l = Some b -> l = make b p.
+  Proof.
+    unfold get_pol.
+    intros.
+    destruct (p =? var l)%positive eqn:E.
+    inv H.
+    rewrite Pos.eqb_eq in E.
+    subst.
+    apply decomp.
+    discriminate.
+  Qed.
+
+  Lemma get_pol_None : forall p l,
+      get_pol p l = None -> var l <> p.
+  Proof.
+    unfold get_pol.
+    intros.
+    destruct (p =? var l)%positive eqn:E.
+    discriminate.
+    apply Pos.eqb_neq in E.
+    congruence.
+  Qed.
+
+  Lemma eval_lit_negb_make : forall env b p,
+      beval_lit env (make b p) = negb (beval_lit env (make (negb b) p)).
+  Proof.
+    unfold beval_lit. unfold make.
+    destruct b; simpl;auto.
+    intros. rewrite negb_involutive. reflexivity.
+  Qed.
+
+  Lemma make_var : forall b a,
+      make b (var a) <> a -> make (negb b) (var a) = a.
+  Proof.
+    unfold make.
+    destruct b,a; simpl; congruence.
+  Qed.
+
+  
+End Lit.
+Import Lit.
+
+
+Definition clause := list Lit.t.
+
+Fixpoint cons_lit (l:Lit.t) (cl:clause) :=
+  match cl with
+  | nil => l::nil
+  | l1::cl' => if pol l1 || negb (pol l) then l::cl
+               else l1 ::(cons_lit l cl')
+  end.
+
+Lemma cons_lit_POS_true : forall l cl,
+    pol l = true ->
+    cons_lit l (map POS cl) = POS (var l) :: map POS cl.
+Proof.
+  induction cl.
+  - simpl. intros. destruct l; simpl ; auto. discriminate.
+  - intros. simpl.  destruct l; simpl ; auto. discriminate.
+Qed.
+
+Lemma cons_lit_POS_false : forall l cl,
+    pol l = false ->
+    cons_lit l cl = l :: cl.
+Proof.
+  induction cl;simpl.
+  - reflexivity.
+  - intros.
+    rewrite H. rewrite orb_comm. simpl.
+    reflexivity.
+Qed.
+
+Definition wf (l : clause) :=
+  exists l1 l2, l=(List.map NEG l1) ++ (List.map POS l2).
+
+Lemma sublist_forall : forall {A: Type} (P : A -> Prop) l1 l2,
+    Forall P l2 ->
+    sublist l1 l2 ->
+    Forall P l1.
+Proof.
+  intros.
+  induction H0.
+  constructor.
+  inv H.
+  tauto.
+  inv H.
+  constructor; auto.
+Qed.
+
+Lemma wf_sublist :
+  forall cl cl'
+           (SUB:sublist cl' cl)
+           (WF: wf cl),
+      wf cl'.
+  Proof.
+    unfold wf.
+    intros.
+    destruct WF as (n & p & EQ).
+    revert n p EQ.
+    induction SUB;intros.
+    - exists nil. exists nil. reflexivity.
+    - destruct n.
+      destruct p.
+      + discriminate.
+      + inv EQ.
+        destruct (IHSUB nil p0 eq_refl) as (n1& n2 & EQ).
+        subst.
+        exists n1. exists n2.
+        reflexivity.
+      + inv EQ.
+        destruct (IHSUB _ _ eq_refl) as (n1& n2 & EQ).
+        subst.
+        exists n1. exists n2.
+        reflexivity.
+    - destruct n.
+      destruct p.
+      + discriminate.
+      + inv EQ.
+        destruct (IHSUB nil p0 eq_refl) as (n1& n2 & EQ).
+        subst.
+        destruct n1.
+        * simpl. exists nil,(p::n2). reflexivity.
+        * simpl in SUB.
+          apply (sublist_forall Lit.isPOS) in SUB.
+          inv SUB. discriminate.
+          rewrite Forall_map.
+          rewrite Forall_forall.
+          intros. reflexivity.
+      + inv EQ.
+        destruct (IHSUB _ _ eq_refl) as (n1& n2 & EQ).
+        subst.
+        exists (p0::n1).
+        exists n2.
+        reflexivity.
+  Qed.
+
+
+
+Lemma wf_cons_lit : forall l cl,
+    wf cl -> wf (cons_lit l cl).
+Proof.
+  unfold wf.
+  intros.
+  destruct H as (l1 & l2 & EQ).
+  subst.
+  revert l2.
+  induction l1.
+  - simpl. intros.
+    destruct (pol l) eqn:POL.
+    exists nil,(var l::l2).
+    rewrite cons_lit_POS_true by auto.
+    reflexivity.
+    exists (var l::nil),l2.
+    simpl.
+    rewrite cons_lit_POS_false by auto.
+    destruct l ; try discriminate ; reflexivity.
+  - intros.
+    simpl.
+    destruct (pol l) eqn:PL; simpl.
+    destruct (IHl1 l2) as (l1' & l2' & EQ).
+    rewrite EQ.
+    exists (a::l1'), l2'.
+    reflexivity.
+    exists (var l ::a ::l1), l2.
+    destruct l; try discriminate. reflexivity.
+Qed.
+
+
+Fixpoint eval_clause (env : positive -> Prop) (cl : clause) :=
+  match cl with
+  | nil => False
+  | e::cl' => eval_lit env e (eval_clause env cl')
+  end.
+
+Fixpoint beval_clause (env : positive -> bool) (cl : clause) :=
+  match cl with
+  | nil => false
+  | e::cl' => beval_lit env e || beval_clause env cl'
+  end.
+
+Definition cnf := list clause.
+
+Definition beval_cnf (env :positive -> bool) (l: cnf) :=
+  List.fold_right (fun e acc => beval_clause env e && acc) true l.
+
+Definition eval_cnf (env :positive -> Prop) (l: cnf) :=
+  List.fold_right (fun e acc => eval_clause env e /\ acc) True l.
+
+
+Lemma beval_clause_app : forall env l1 l2,
+    beval_clause env (l1 ++ l2) = (beval_clause env l1 || beval_clause env l2).
+Proof.
+  induction l1; simpl.
+  - reflexivity.
+  - intros.
+    rewrite IHl1.
+    btauto.
+Qed.
+
+Lemma beval_cnf_app : forall env l1 l2,
+    beval_cnf env (l1 ++ l2) = (beval_cnf env l1 && beval_cnf env l2).
+Proof.
+  induction l1; simpl.
+  - tauto.
+  - intros.
+    rewrite IHl1.
+    btauto.
+Qed.
+
+Lemma eval_cnf_app : forall env l1 l2,
+    eval_cnf env (l1 ++ l2) <-> (eval_cnf env l1 /\ eval_cnf env l2).
+Proof.
+  induction l1; simpl.
+  - tauto.
+  - intros.
+    rewrite IHl1.
+    tauto.
+Qed.
+
+
+Inductive has_cardinal {A: Type}: list A -> nat -> Prop :=
+| Card0 : has_cardinal nil 0
+| CardS : forall n l x, has_cardinal l n ->
+                        ~ In x l ->
+                        has_cardinal (x::l) (S n).
+
+Lemma has_cardinal_no_dup : forall {A: Type} (l:list A),
+    NoDup l ->
+    has_cardinal l (length l).
+Proof.
+  intros.
+  induction H.
+  - simpl. constructor.
+  - simpl.
+    constructor;auto.
+Qed.
+
+Definition vars_of_clause (cl:clause) := List.map Lit.var cl.
+
+Definition vars_of_cnf (cls : cnf) := List.fold_right (fun e acc => vars_of_clause e ++ acc) nil cls.
+
+Lemma nodup_nil : forall {A: Type} (dec : forall (x y:A), {x = y} + {x <> y}) l,
+                         nodup dec l = nil -> l = nil.
+Proof.
+  induction l.
+  - reflexivity.
+  - simpl. destruct (in_dec dec a l).
+    intro. apply IHl in H. subst. simpl in i. tauto.
+    discriminate.
+Qed.
+
+Lemma vars_of_clause_nil : forall l, vars_of_clause l = nil -> l = nil.
+Proof.
+  unfold vars_of_clause.
+  apply map_eq_nil.
+Qed.
+
+Lemma vars_of_cnf_nil : forall cls,
+    vars_of_cnf cls = nil ->
+    cls = List.map (fun _ => nil) cls.
+Proof.
+  induction cls.
+  - simpl. reflexivity.
+  - simpl. intros.
+    apply app_eq_nil in H.
+    destruct H as [H1 H2].
+    apply vars_of_clause_nil in H1.
+    apply IHcls in H2.
+    subst a. rewrite <- H2. reflexivity.
+Qed.
+
+Definition is_clause_of (p:positive) (cl: list Lit.t) :=
+  forall l, In l cl -> var l = p.
+
+Lemma vars_of_cnf_uniq : forall p cls,
+  (forall x : positive, In x (vars_of_cnf cls) -> x = p) ->
+  forall cl : clause, In cl cls -> is_clause_of p cl.
+Proof.
+  induction cls.
+  - intros. simpl in H0. tauto.
+  - intros.
+    simpl in H0. simpl in H. destruct H0 ; subst.
+    assert ((forall x, In x (vars_of_clause cl) -> x = p)).
+    { intros. apply H. rewrite in_app_iff. tauto. }
+    clear H IHcls.
+    unfold is_clause_of.
+    intros. unfold vars_of_clause in H0. apply H0.
+    rewrite in_map_iff. exists l; simpl;auto.
+    eapply IHcls;eauto.
+    intros.
+    apply H. rewrite in_app_iff. tauto.
+Qed.
+
+Definition boeval (env : positive -> bool) (o: option positive) :=
+  match o with
+  | None => false
+  | Some i => env i
+  end.
+
+Definition oeval (env: positive -> Prop) (o: option positive) :=
+  match o with
+  | None => False
+  | Some i => env i
+  end.
+
+
+Fixpoint map_filter {A B: Type} (F: A -> option B ) (l: list A) : list B :=
+  match l with
+  | nil => nil
+  | e::l => match F e with
+            | None => map_filter F l
+            | Some e' => e' :: map_filter F l
+            end
+  end.
+
+
+Module Elim.
+
+  Fixpoint get_polarity_rec (p:positive)  (l :  clause) :=
+    match l with
+    | nil => None
+    | li :: l => match Lit.get_pol p li with
+                 | None =>
+                     match get_polarity_rec p  l with
+                     | None => None
+                     | Some (b,l) => Some (b,li::l)
+                     end
+                 | Some b   => Some (b,l)
+                 end
+    end.
+
+  Fixpoint normalise (cl: clause): option clause :=
+    match cl with
+    | nil => Some nil
+    | l::cl' => match normalise cl' with
+                | None => None
+                | Some cl' => match get_polarity_rec (Lit.var l) cl'  with
+                              | None => Some (l::cl')
+                              | Some(b,_) => if Lit.eq_dec (Lit.make (negb b) (Lit.var l)) l
+                                             then None else Some cl'
+                              end
+                end
+    end.
+
+  Fixpoint split_clause (l1: clause) : clause * clause :=
+    match  l1 with
+    | nil => (nil,nil)
+    | POS p::l => (nil,l1)
+    | NEG p::l => let (ln,lp):= split_clause l in
+                  (NEG p::ln,lp)
+    end.
+
+
+  Definition merge_clause (cl1 cl2 : clause) : clause :=
+    let (cln1,clp1) := split_clause cl1 in
+    let (cln2,clp2) := split_clause cl2 in
+    cln1 ++ cln2 ++ clp1 ++ clp2.
+
+
+Fixpoint resolve_all (l1:cnf) (l2:cnf) :=
+  match l1 with
+  | nil => nil
+  | cl::l1 => map_filter normalise (List.map (merge_clause cl) l2) ++ (resolve_all l1 l2)
+  end.
+
+
+
+Fixpoint split_polarity (p: positive) (l: cnf) : cnf * cnf * cnf:=
+  match l with
+  | nil => (nil,nil,nil)
+  | cl::l => let '(lp,ln,lo) := split_polarity p l in
+             match normalise cl with
+             | None => split_polarity p l
+             | Some cl' =>
+                 match get_polarity_rec p cl' with
+                 | None => (lp,ln,cl'::lo)
+                 | Some(b,cl') => (if b then cl'::lp else lp ,if b then ln else cl'::ln,lo)
+                 end
+             end
+  end.
+
+
+Definition elim (p:positive) (l: cnf) :=
+  let '(lp,ln,lo) := split_polarity p l in
+  resolve_all lp ln ++ lo.
+
+
+(*  Definition eval_oclause (env: positive -> Prop) (cl:option clause) :=
+    match cl with
+    | None => True
+    | Some cl => eval_clause env cl
+    end.
+*)
+
+
+End Elim.
+
+
+Definition is_var_of_clause (v:positive) (cl: clause) :=
+  exists l, In l cl /\ var l = v.
+
+Definition is_var_of_cnf (v:positive) (cls: cnf) :=
+  exists cl, In cl cls /\ is_var_of_clause v cl.
+
+Lemma is_var_of_cnf_cons : forall v c cls,
+    is_var_of_cnf v (c :: cls) <-> (is_var_of_clause v c \/ is_var_of_cnf v cls).
+Proof.
+  unfold is_var_of_cnf at 1.
+  intros. simpl. firstorder congruence.
+Qed.
+
+Lemma is_var_of_cnf_nil : forall v,
+    is_var_of_cnf v nil <-> False.
+Proof.
+  unfold is_var_of_cnf at 1.
+  intros. simpl. firstorder congruence.
+Qed.
+
+Lemma is_var_of_cnf_app : forall v cl1 cl2,
+    is_var_of_cnf v (cl1 ++cl2) <-> (is_var_of_cnf v cl1 \/ is_var_of_cnf v cl2).
+Proof.
+  induction cl1.
+  - intros.
+    simpl.
+    rewrite is_var_of_cnf_nil.
+    tauto.
+  -intros.
+   simpl.
+   rewrite !is_var_of_cnf_cons.
+   rewrite IHcl1.
+   tauto.
+Qed.
+
+
+
+
+Lemma is_var_of_clause_cons : forall v l cl,
+    is_var_of_clause v (l::cl) <->
+      var l = v \/ is_var_of_clause v cl.
+Proof.
+  unfold is_var_of_clause.
+  simpl. firstorder congruence.
+Qed.
+
+Lemma is_var_of_clause_nil : forall v,
+    is_var_of_clause v nil <-> False.
+Proof.
+  unfold is_var_of_clause.
+  simpl. firstorder congruence.
+Qed.
+
+Lemma is_var_of_clause_app : forall v cl1 cl2,
+    is_var_of_clause v (cl1++cl2) <->
+      is_var_of_clause v cl1 \/ is_var_of_clause v cl2.
+Proof.
+  induction cl1;simpl;intros.
+  - rewrite is_var_of_clause_nil.
+  tauto.
+  - rewrite! is_var_of_clause_cons.
+    rewrite! IHcl1.
+    tauto.
+Qed.
+
+
+
+
+
+Lemma vars_of_clause_ok : forall p cl,
+    is_var_of_clause p cl <-> In p (vars_of_clause cl).
+Proof.
+  induction cl.
+  - rewrite is_var_of_clause_nil.
+    simpl. tauto.
+  - rewrite is_var_of_clause_cons.
+    simpl.
+    rewrite IHcl.
+    tauto.
+Qed.
+
+Lemma vars_of_cnf_ok : forall cls v,
+    is_var_of_cnf v cls <-> In v (vars_of_cnf cls).
+Proof.
+  unfold is_var_of_cnf, vars_of_cnf,vars_of_clause.
+  induction cls;simpl;intros.
+  - split; firstorder.
+  - rewrite in_app_iff.
+    rewrite <- IHcls.
+    rewrite in_map_iff.
+    firstorder congruence.
+Qed.
+
+Lemma is_var_of_cnf_False : forall cls,
+    (forall v : positive, is_var_of_cnf v cls -> False) ->
+    forall cl, In cl cls -> cl = nil.
+Proof.
+  intros.
+  induction cls.
+  - simpl. firstorder.
+  - simpl in H0.
+    destruct H0; subst.
+    destruct cl;auto.
+    exfalso.
+    apply (H (var t0)).
+    rewrite is_var_of_cnf_cons.
+    left. rewrite is_var_of_clause_cons.
+    tauto.
+    eapply IHcls; auto.
+    intros.
+    apply (H v).
+    rewrite is_var_of_cnf_cons. tauto.
+Qed.
+
+Definition match_option (p:positive) (o:option positive) :=
+  match o with
+  | None => False
+  | Some q => p = q
+  end.
+
+Lemma match_option_dec : forall p o,
+    match_option p o \/ ~ match_option p o.
+Proof.
+  destruct o; simpl.
+  destruct (Pos.eq_dec p p0);tauto.
+  tauto.
+Qed.
+
+Lemma beval_clauses_Nil : forall p,
+    (forall env : positive -> bool,
+        beval_cnf env nil = true -> env p = true) -> False.
+Proof.
+  intros.
+  simpl in H.
+  specialize (H (fun _ => false) eq_refl).
+  discriminate.
+Qed.
+
+
+Lemma beval_clause_one_var : forall p cl,
+  (forall v : positive, is_var_of_clause v cl -> p = v) ->
+  beval_clause (fun _ => false) cl = false ->
+  (forall l, In l cl -> l = POS p).
+Proof.
+  intros.
+  induction cl.
+  - simpl in *.
+    tauto.
+  - simpl in *.
+    rewrite orb_false_iff in *.
+    destruct H0 ; subst.
+    intros.
+    destruct H1 ; subst.
+     +
+    assert (p = (var l)).
+    {
+      apply H.  unfold is_var_of_clause.
+      simpl. exists l. intuition congruence.
+    }
+    subst.
+    destruct l ; simpl in *; auto.
+    unfold beval_lit in *.
+    simpl in *. discriminate.
+     +
+       eapply IHcl; eauto.
+       intros.
+       apply H.
+       rewrite is_var_of_clause_cons.
+       tauto.
+Qed.
+
+Lemma beval_clauses_one_var : forall p cls,
+  (forall env : positive -> bool,
+    beval_cnf env cls = true -> env p = true) ->
+  (forall v : positive, is_var_of_cnf v cls -> p = v) ->
+  exists cl, In cl cls /\ forall l, In l cl -> l = POS p.
+Proof.
+  intros.
+  specialize (H (fun _ => false)).
+  induction cls.
+  - simpl in *.
+    intuition congruence.
+  - simpl in *.
+    destruct (beval_clause (fun _ : positive => false) a) eqn:B.
+    simpl in H.
+    apply IHcls in H.
+    destruct H as (cl & IN & ALLPOS).
+    exists cl.
+    tauto.
+    { intros. apply H0.
+      rewrite is_var_of_cnf_cons. tauto.
+    }
+    simpl in H.
+    clear H.
+    assert (IVC : forall v : positive, is_var_of_clause v a -> p = v).
+    { intros. apply H0. rewrite is_var_of_cnf_cons. tauto. }
+    specialize (beval_clause_one_var p _ IVC B).
+    intros.
+    exists a. tauto.
+Qed.
+
+Lemma eval_clause_POS : forall env p cl,
+  (forall l : t, In l cl -> l = POS p) ->
+  eval_clause env cl ->
+  env p.
+Proof.
+  induction cl; simpl.
+  - tauto.
+  - intros.
+    unfold eval_lit in H0.
+    rewrite (H _ (or_introl eq_refl)) in *.
+    simpl in H0.
+    destruct H0;auto.
+Qed.
+
+Lemma eval_clauses_all_pos :
+  forall env p cl cls
+         (INC : In cl cls)
+         (ALLP : forall l : t, In l cl -> l = POS p),
+    eval_cnf env cls -> env p.
+Proof.
+  induction cls.
+  - simpl. tauto.
+  - intros.
+    simpl in H. destruct H.
+    destruct INC. subst.
+    eapply eval_clause_POS in ALLP; eauto.
+    eapply IHcls; eauto.
+Qed.
+
+Lemma eval_clause_cons_lit_POS : forall env l cl,
+    Forall (fun l : t => pol l = true) cl ->
+    eval_lit env l (eval_clause env cl) <-> eval_clause env (cons_lit l cl).
+Proof.
+  intros. induction H.
+  - simpl. tauto.
+  - simpl. rewrite H. simpl.
+    tauto.
+Qed.
+
+Lemma eval_clause_cons_lit_NEG : forall env l cl,
+    pol l = false ->
+    eval_lit env l (eval_clause env cl) <-> eval_clause env (cons_lit l cl).
+Proof.
+  intros. induction cl; simpl.
+  - simpl. tauto.
+  - rewrite H. simpl. rewrite orb_comm. simpl.
+    tauto.
+Qed.
+
+
+
+Lemma beval_clause_cons_lit : forall env l cl,
+    beval_clause env (cons_lit l cl) = (beval_lit env l || beval_clause env cl).
+Proof.
+  induction cl; simpl.
+  - reflexivity.
+  - destruct (pol a || (negb (pol l))).
+    simpl. btauto.
+    simpl. rewrite IHcl. btauto.
+Qed.
+
+Lemma get_polarity_spec :
+  forall env p cl,
+         match Elim.get_polarity_rec p cl with
+         | None => ~ is_var_of_clause  p  cl
+         | Some (b,cl') =>
+             beval_clause env cl = beval_clause env (cons_lit (Lit.make b p) cl')
+         end.
+Proof.
+  induction cl.
+  - simpl. rewrite is_var_of_clause_nil. tauto.
+  - intros.
+    simpl.
+    destruct (Lit.get_pol p a) eqn:GP.
+    apply Lit.get_pol_inv in GP.
+    subst.
+    + rewrite beval_clause_cons_lit.
+      reflexivity.
+    + destruct (Elim.get_polarity_rec p cl).
+      destruct p0.
+      rewrite beval_clause_cons_lit in *.
+      rewrite IHcl.
+      simpl.
+      rewrite orb_comm.
+      rewrite <- orb_assoc.
+      f_equal.
+      rewrite orb_comm.
+      reflexivity.
+      * rewrite is_var_of_clause_cons.
+        apply Lit.get_pol_None in GP.
+        intro. intuition congruence.
+Qed.
+
+Definition beval_option {A: Type} (eA: A -> bool) (v: option A) :=
+  match v with
+  | None => true
+  | Some v => eA v
+  end.
+
+Definition eval_option {A: Type} (eA: A -> Prop) (v: option A) :=
+  match v with
+  | None => True
+  | Some v => eA v
+  end.
+
+
+Lemma beval_normalise : forall env cl,
+    beval_clause env cl = beval_option (beval_clause env) (Elim.normalise cl).
+Proof.
+  induction cl.
+  - simpl. reflexivity.
+  - simpl.
+    destruct (Elim.normalise cl) eqn:N.
+    simpl in *.
+    rewrite IHcl.
+    generalize (get_polarity_spec env (var a) c).
+    destruct (Elim.get_polarity_rec (Lit.var a) c) eqn:GP.
+    destruct p.
+    destruct (Lit.eq_dec (Lit.make (negb b) (Lit.var a)) a).
+    +
+      rewrite beval_clause_cons_lit.
+      simpl.
+      intro E.
+      rewrite E.
+      rewrite <- e at 1.
+      rewrite orb_assoc.
+      rewrite eval_lit_negb_make.
+      rewrite negb_involutive.
+      rewrite orb_negb_l. reflexivity.
+    + intros.
+      simpl.
+      rewrite H.
+      rewrite beval_clause_cons_lit.
+      simpl.
+      apply make_var in n.
+      rewrite negb_involutive in n.
+      rewrite n.
+      btauto.
+    + simpl.
+      auto.
+    + simpl in *.
+      rewrite IHcl.
+      btauto.
+Qed.
+
+Lemma beval_cnf_cons_lit : forall env l lp,
+    beval_cnf env (map (cons_lit l) lp) = (Lit.beval_lit env l || (beval_cnf env lp)).
+Proof.
+  induction lp;simpl.
+  - btauto.
+  - rewrite IHlp.
+    rewrite beval_clause_cons_lit.
+    btauto.
+Qed.
+
+
+Lemma split_polarity_eval : forall env p l lp ln lo,
+    Elim.split_polarity p l = (lp,ln,lo) ->
+    beval_cnf env l = (beval_cnf env lo) && (beval_cnf env (List.map (cons_lit (Lit.POS p)) lp))
+                      && (beval_cnf env (List.map (cons_lit (Lit.NEG p)) ln)).
+Proof.
+  induction l.
+  - simpl; intros.
+    inv H.
+    simpl. reflexivity.
+  -  intros.
+     simpl in H.
+     simpl.
+     destruct (Elim.split_polarity p l) as [[lp' ln'] lo'] eqn:E.
+     rewrite (IHl lp' ln' lo') by auto.
+     rewrite (beval_normalise env a).
+     destruct (Elim.normalise a); simpl.
+     +
+       generalize (get_polarity_spec env p c).
+       destruct (Elim.get_polarity_rec p c).
+       destruct p0 as [b cl'].
+       inv H.
+       intros.
+       rewrite H.
+       rewrite !beval_cnf_cons_lit. simpl.
+       rewrite beval_clause_cons_lit.
+       destruct b ; simpl.
+       btauto.
+       btauto.
+       inv H.
+       intros.
+       simpl.
+       btauto.
+     +  inv H. btauto.
+Qed.
+
+Lemma beval_cnf_normalise : forall env cl,
+    beval_cnf env (map_filter Elim.normalise cl) =  beval_cnf env cl.
+Proof.
+  induction cl.
+  - simpl. tauto.
+  - simpl.
+    specialize (beval_normalise env a).
+    destruct (Elim.normalise a).
+    simpl. intro. rewrite <- H. rewrite IHcl. reflexivity.
+    simpl. intros. rewrite H. simpl. auto.
+Qed.
+
+Lemma beval_split_clause : forall env cl1 n1 p1,
+    Elim.split_clause cl1 = (n1, p1) ->
+    beval_clause env cl1 = beval_clause env(n1 ++ p1).
+Proof.
+  induction cl1.
+  - simpl. intros. inv H.
+    reflexivity.
+  - intros. simpl in H.
+    destruct a. inv H.
+    simpl. reflexivity.
+    destruct (Elim.split_clause cl1) as (ln2,lp2) eqn:SC.
+    inv H.
+    simpl. erewrite IHcl1; eauto.
+Qed.
+
+Lemma beval_merge_clause : forall env cl1 cl2,
+    beval_clause env (Elim.merge_clause cl1 cl2) = (beval_clause env cl1 || beval_clause env cl2).
+Proof.
+  unfold Elim.merge_clause.
+  intros.
+  destruct (Elim.split_clause cl1) as (cln1,clp1) eqn:SC1.
+  destruct (Elim.split_clause cl2) as (cln2,clp2) eqn:SC2.
+  rewrite! beval_clause_app.
+  eapply beval_split_clause in SC1;eauto.
+  eapply beval_split_clause in SC2;eauto.
+  rewrite SC1. rewrite SC2.
+  rewrite! beval_clause_app.
+  btauto.
+Qed.
+
+
+Lemma beval_cnf_merge_clause : forall env clp ln,
+    beval_cnf env (map (Elim.merge_clause clp) ln) = beval_clause env clp || beval_cnf env ln.
+Proof.
+  induction ln.
+  - simpl. rewrite orb_comm. reflexivity.
+  - simpl.
+    rewrite IHln.
+    rewrite beval_merge_clause.
+    btauto.
+Qed.
+
+Lemma beval_cnf_Forall : forall env cls,
+    beval_cnf env cls = true <->
+    Forall (fun x : clause => beval_clause env x = true) cls.
+Proof.
+  induction cls.
+  - simpl; split; auto.
+  - simpl. rewrite andb_true_iff.
+    rewrite IHcls.
+    intuition. inv H1; auto.
+    inv H1; auto.
+Qed.
+
+
+Lemma resolve_all_eval : forall env lp ln,
+        beval_cnf  env (Elim.resolve_all lp ln)= true ->
+        forall clp cln, In clp lp -> In cln ln -> beval_clause env clp = true \/ beval_clause env cln = true.
+Proof.
+  induction lp;simpl.
+  - tauto.
+  - intros.
+    rewrite beval_cnf_app in H.
+    rewrite andb_true_iff in H.
+    destruct  H as [E1 E2].
+    destruct H0 ; subst.
+    rewrite beval_cnf_normalise in E1.
+    rewrite beval_cnf_merge_clause in E1.
+    rewrite orb_true_iff in E1.
+    destruct E1 ; auto.
+    right.
+    revert cln H1.
+    rewrite <- Forall_forall.
+    apply beval_cnf_Forall;auto.
+    eapply IHlp;eauto.
+Qed.
+
+Lemma NoDup_no_var :
+  forall p c
+         (ND : NoDup (vars_of_clause c)) b c',
+    Elim.get_polarity_rec p c = Some (b, c') ->
+    is_var_of_clause p c' ->
+    False.
+Proof.
+  induction c.
+  - intros. simpl in H. discriminate.
+  - intros. simpl in ND.
+    inv ND.
+    simpl in H.
+    destruct (get_pol p a) eqn:POL.
+    + inv H.
+    apply get_pol_inv in POL.
+    subst.
+    rewrite Lit.var_make in H3.
+    rewrite <- vars_of_clause_ok in H3.
+    tauto.
+    +  apply get_pol_None in POL.
+       destruct (Elim.get_polarity_rec p c) eqn:GP; try discriminate.
+       destruct p0. inv H.
+       rewrite is_var_of_clause_cons in H0.
+       destruct H0; try tauto.
+       eapply IHc;eauto.
+Qed.
+
+Lemma normalise_NoDup : forall a c,
+    Elim.normalise a = Some c ->
+    NoDup (vars_of_clause c).
+Proof.
+  induction a.
+  - simpl. intros. inv H. constructor.
+  - simpl. intros.
+    destruct (Elim.normalise a0) eqn:N.
+    destruct (Elim.get_polarity_rec (var a) c0) eqn:GP.
+    destruct p. destruct (eq_dec (make (negb b) (var a)) a).
+    +  discriminate.
+    + inv H.
+      apply IHa; auto.
+    +inv H.
+     simpl.
+     constructor.
+     generalize (get_polarity_spec (fun _ => true) (var a) c0).
+     rewrite GP.
+     rewrite vars_of_clause_ok. auto.
+     apply IHa;auto.
+    +  discriminate.
+Qed.
+
+Lemma split_polarity_vars :
+  forall p l lp ln lo,
+    Elim.split_polarity p l = (lp,ln,lo) ->
+    ~ is_var_of_cnf p lp /\ ~ is_var_of_cnf p ln /\ ~ is_var_of_cnf p lo.
+Proof.
+  induction l ;simpl.
+  - intros. inv H.
+    rewrite is_var_of_cnf_nil.
+    tauto.
+  - intros.
+    destruct (Elim.split_polarity p l) as [[lp' ln'] lo'] eqn:SP.
+    destruct (Elim.normalise a) eqn:NORM.
+    specialize (IHl _ _ _  eq_refl).
+    destruct (Elim.get_polarity_rec p c) eqn:P.
+    destruct p0. inv H.
+    assert (~ is_var_of_clause p l0).
+    { intro.
+      eapply NoDup_no_var in P; auto.
+      eapply normalise_NoDup in NORM    ; eauto.
+    }
+    destruct b; rewrite is_var_of_cnf_cons.
+    tauto. tauto.
+    inv H.
+    rewrite is_var_of_cnf_cons.
+    specialize (get_polarity_spec (fun _ => true) p c).
+    rewrite P.
+    tauto.
+    inv H. eapply IHl;eauto.
+Qed.
+
+Definition set_env {A: Type}(env: positive -> A) (x': positive) (v: A) :=
+  fun x => if Pos.eq_dec x x' then v else env x.
+
+Lemma set_env_same : forall {A:Type} env p (v:A),
+    set_env env p v p = v.
+Proof.
+  unfold set_env.
+  intros. destruct (Pos.eq_dec p p);try congruence.
+Qed.
+
+Lemma beval_lit_no_var : forall p b env l,
+    var l <> p ->
+    beval_lit (set_env env p b) l = beval_lit env l.
+Proof.
+  unfold beval_lit.
+  intros.
+  unfold set_env.
+  destruct (Pos.eq_dec (var l) p); try congruence.
+Qed.
+
+Lemma beval_clause_no_var : forall p b env cl,
+    ~ is_var_of_clause p cl ->
+    beval_clause (set_env env p b) cl = beval_clause env cl.
+Proof.
+  induction cl;simpl.
+  - reflexivity.
+  - rewrite is_var_of_clause_cons.
+    intros.
+    rewrite IHcl by tauto.
+    rewrite beval_lit_no_var by tauto.
+    reflexivity.
+Qed.
+
+Lemma beval_no_var : forall p l b env,
+    ~ is_var_of_cnf p  l ->
+    beval_cnf (set_env env p b) l = beval_cnf env l.
+Proof.
+  intros.
+  induction l.
+  - simpl. reflexivity.
+  - simpl.
+    rewrite is_var_of_cnf_cons in H.
+    rewrite IHl by tauto.
+    f_equal.
+    apply beval_clause_no_var.
+    tauto.
+Qed.
+
+Lemma beval_cnf_exists : forall env cls,
+    (beval_cnf env cls = true -> False) ->
+    exists cl, In cl cls /\ beval_clause env cl = false.
+Proof.
+  induction cls;simpl.
+  - tauto.
+  - intros.
+    rewrite andb_true_iff in H.
+    destruct (beval_clause env a) eqn:EC.
+    specialize (fun E => H (conj eq_refl E)).
+    apply IHcls in H.
+    destruct H as (c & T1 & T2).
+    exists c. tauto.
+    exists a. tauto.
+Qed.
+
+
+Lemma elim_complete :
+  forall p l
+         (EV :forall env , beval_cnf env l = true -> False)
+         env
+         (EL : beval_cnf env  (Elim.elim p l) = true), False.
+    Proof.
+      unfold Elim.elim.
+      intros.
+      destruct (Elim.split_polarity p l) as [[lp ln] lo] eqn:SP.
+      rewrite beval_cnf_app in EL.
+      assert (EV' : forall env, beval_cnf env lo && beval_cnf env (map (cons_lit (POS p)) lp) && beval_cnf env (map (cons_lit (NEG p)) ln) = true -> False).
+      {
+        intros.
+        apply (EV env0).
+        rewrite (split_polarity_eval env0 p l lp ln lo) by auto.
+        tauto.
+      }
+      clear EV.
+      rewrite andb_true_iff in EL.
+      destruct EL as (EL1 & EL2).
+      apply split_polarity_vars in SP ; auto.
+      generalize (EV' (set_env env p true)).
+      generalize (EV' (set_env env p false)).
+      clear EV'.
+      rewrite! beval_cnf_cons_lit.
+      unfold beval_lit; simpl.
+      rewrite! set_env_same. simpl.
+      rewrite! andb_true_r.
+      rewrite! beval_no_var by tauto.
+      rewrite EL2.
+      simpl.
+      intros.
+      apply beval_cnf_exists in H.
+      apply beval_cnf_exists in H0.
+      destruct H as (cl1 & IN1 & E1).
+      destruct H0 as (cl2 & IN2 & E2).
+      eapply resolve_all_eval in EL1;eauto.
+      intuition congruence.
+    Qed.
+
+    Definition clause_of_opt (o:option positive) :=
+      match o with
+      | None => nil
+      | Some i => (NEG i :: nil) ::nil
+      end.
+
+    Lemma eval_clause_of_opt : forall env l,
+        beval_cnf env (clause_of_opt l) = negb (boeval env l).
+    Proof.
+      destruct l;simpl.
+      unfold beval_lit. simpl.
+      btauto.
+      reflexivity.
+    Qed.
+
+    Lemma neg_concl : forall cls l,
+      (forall env, beval_cnf env cls = true -> boeval env l = true)
+      <->
+        (forall env, beval_cnf env (clause_of_opt l ++ cls) = true -> False).
+    Proof.
+      split;intros.
+      rewrite beval_cnf_app in *.
+      rewrite andb_true_iff in H0.
+      destruct H0.
+      apply H in H1.
+      rewrite eval_clause_of_opt in H0.
+      rewrite H1 in H0. discriminate.
+      specialize (H env).
+      rewrite beval_cnf_app in H.
+      rewrite eval_clause_of_opt in H.
+      destruct (boeval env l); auto.
+    Qed.
+
+    Lemma get_polarity_spec_var : forall p c,
+        Elim.get_polarity_rec p c <> None ->
+        is_var_of_clause p c.
+    Proof.
+      induction c ; simpl.
+      - rewrite is_var_of_clause_nil.
+        tauto.
+      - destruct (get_pol p a) eqn: POL.
+        rewrite is_var_of_clause_cons.
+        intros.
+        apply get_pol_inv in POL.
+        subst.
+        rewrite var_make. tauto.
+        destruct (Elim.get_polarity_rec p c); try congruence.
+        destruct p0.
+        intros.
+        apply get_pol_None in POL.
+        rewrite is_var_of_clause_cons.
+        intuition congruence.
+    Qed.
+
+    Lemma get_polarity_spec_not_var : forall p c,
+        ~ is_var_of_clause p c ->
+        Elim.get_polarity_rec p c = None.
+    Proof.
+      intros.
+      destruct (Elim.get_polarity_rec p c) eqn:G;auto.
+      exfalso.
+      assert (Elim.get_polarity_rec p c <> None) by congruence.
+      apply get_polarity_spec_var in H0.
+      tauto.
+    Qed.
+
+
+    Lemma normalise_vars : forall p c c',
+        Elim.normalise c = Some c' ->
+        is_var_of_clause p c <-> is_var_of_clause p c'.
+    Proof.
+      induction c;simpl.
+      - intros. inv H.
+        tauto.
+      - intros.
+        destruct (Elim.normalise c) eqn: N; try discriminate.
+        destruct (Elim.get_polarity_rec (var a) c0) eqn: G.
+        destruct p0.
+        destruct (eq_dec (make (negb b) (var a)) a); try discriminate.
+        inv H. rewrite is_var_of_clause_cons.
+        apply make_var in n.
+        rewrite negb_involutive in n.
+        rewrite IHc by auto.
+        assert (G' : Elim.get_polarity_rec (var a) c' <> None) by congruence.
+        apply get_polarity_spec_var  in G'.
+        intuition congruence.
+        inv H.
+        rewrite! is_var_of_clause_cons.
+        rewrite IHc by auto.
+        tauto.
+    Qed.
+
+
+    Lemma split_polarity_no_vars : forall p cl1 cl2 lp ln lo,
+        ~ is_var_of_cnf p cl1 ->
+          Elim.split_polarity p cl2 = (lp,ln,lo) ->
+          Elim.split_polarity p (cl1 ++ cl2) = (lp, ln, map_filter Elim.normalise cl1++lo).
+    Proof.
+      induction cl1.
+      - simpl. auto.
+      - simpl.
+        intros.
+        apply IHcl1 in H0.
+        rewrite H0.
+        destruct (Elim.normalise a) eqn:N.
+        apply normalise_vars with (p:=p) in N.
+        rewrite is_var_of_cnf_cons in H.
+        rewrite get_polarity_spec_not_var by tauto.
+        reflexivity.
+        reflexivity.
+        rewrite is_var_of_cnf_cons in H.
+        tauto.
+    Qed.
+
+    
+Lemma elim_no_vars : forall env p cl1 cl2,
+    ~ is_var_of_cnf p cl1 ->
+    beval_cnf env (Elim.elim p (cl1 ++ cl2)) =     beval_cnf env (cl1 ++ Elim.elim p cl2).
+  Proof.
+    unfold Elim.elim.
+    intros.
+    destruct (Elim.split_polarity p (cl1 ++ cl2)) as ((lp,ln),lo) eqn: S1.
+    destruct (Elim.split_polarity p cl2) as ((lp1,ln1),lo1) eqn: S2.
+    rewrite! beval_cnf_app.
+    apply split_polarity_no_vars with (cl1:=cl1) in S2; auto.
+    rewrite S1 in S2. inv S2.
+    rewrite beval_cnf_app.
+    rewrite beval_cnf_normalise.
+    btauto.
+  Qed.
+
+
+(*Lemma split_polarity_vars :
+  forall p l lp ln lo,
+    Elim.split_polarity p l = (lp,ln,lo) ->
+    (is_var_of_cnf v lp -> is_var_of_cnf v l) /\
+
+Proof.
+  induction l ;simpl.
+  - intros. inv H.
+    rewrite is_var_of_cnf_nil.
+    tauto.
+  - intros.
+    destruct (Elim.split_polarity p l) as [[lp' ln'] lo'] eqn:SP.
+    destruct (Elim.normalise a) eqn:NORM.
+    specialize (IHl _ _ _  eq_refl).
+    destruct (Elim.get_polarity_rec p c) eqn:P.
+    destruct p0. inv H.
+    assert (~ is_var_of_clause p l0).
+    { intro.
+      eapply NoDup_no_var in P; auto.
+      eapply normalise_NoDup in NORM    ; eauto.
+    }
+    destruct b; rewrite is_var_of_cnf_cons.
+    tauto. tauto.
+    inv H.
+    rewrite is_var_of_cnf_cons.
+    specialize (get_polarity_spec (fun _ => true) p c).
+    rewrite P.
+    tauto.
+    inv H. eapply IHl;eauto.
+Qed.
+*)
+  Lemma is_var_of_cnf_normalise : forall v l,
+      is_var_of_cnf v (map_filter Elim.normalise l) ->
+      is_var_of_cnf v l.
+  Proof.
+    induction l; simpl;auto.
+    destruct (Elim.normalise a) eqn: N.
+    - rewrite !is_var_of_cnf_cons.
+      apply normalise_vars with (p:=v) in N.
+      tauto.
+    - rewrite is_var_of_cnf_cons.
+      tauto.
+  Qed.
+
+  Lemma is_var_of_clause_split : forall v cl cln1 clp1,
+      Elim.split_clause cl = (cln1, clp1) ->
+      is_var_of_clause v cl <-> is_var_of_clause  v (cln1 ++clp1).
+  Proof.
+    induction cl;simpl;intros.
+    - inv H. simpl. tauto.
+    - destruct a.
+      inv H.
+      simpl.
+      rewrite! is_var_of_clause_cons.
+      tauto.
+      destruct (Elim.split_clause cl) as (cln2,clp2) eqn:SC1.
+      inv H.
+      rewrite! is_var_of_clause_app.
+      rewrite! is_var_of_clause_cons.
+      rewrite IHcl by reflexivity.
+      rewrite is_var_of_clause_app.
+      tauto.
+  Qed.
+
+
+
+  Lemma is_var_of_clause_merge : forall v cl1 cl2,
+  is_var_of_clause v (Elim.merge_clause cl1 cl2) <->
+    is_var_of_clause v (cl1 ++ cl2).
+  Proof.
+    unfold Elim.merge_clause.
+    intros.
+    destruct (Elim.split_clause cl1) as (cln1,clp1) eqn:SC1.
+    destruct (Elim.split_clause cl2) as (cln2,clp2) eqn:SC2.
+    rewrite! is_var_of_clause_app.
+    apply is_var_of_clause_split with (v:=v) in SC1.
+    apply is_var_of_clause_split with (v:=v) in SC2.
+    rewrite is_var_of_clause_app in *.
+    tauto.
+  Qed.
+
+  Lemma is_var_of_cnf_merge : forall v a l2,
+      is_var_of_cnf v (map (Elim.merge_clause a) l2) ->
+      is_var_of_clause v a \/ is_var_of_cnf v l2.
+  Proof.
+    induction l2.
+    - simpl. rewrite is_var_of_cnf_nil.
+      tauto.
+    - simpl. rewrite! is_var_of_cnf_cons.
+      rewrite! is_var_of_clause_merge.
+      rewrite! is_var_of_clause_app.
+      tauto.
+  Qed.
+
+  Lemma is_var_of_cnf_resolve : forall v l1 l2,
+      is_var_of_cnf v (Elim.resolve_all l1 l2) ->
+        is_var_of_cnf v (l1++ l2).
+  Proof.
+    induction l1;simpl.
+    - intros. rewrite is_var_of_cnf_nil in H. tauto.
+    - intros.
+      rewrite is_var_of_cnf_app in H.
+      destruct H.
+      + rewrite is_var_of_cnf_cons.
+        rewrite or_comm.
+        rewrite is_var_of_cnf_app.
+        rewrite or_assoc.
+        right.
+        apply is_var_of_cnf_normalise in H.
+        apply is_var_of_cnf_merge in H.
+        tauto.
+      + apply IHl1 in H.
+        rewrite is_var_of_cnf_cons.
+        tauto.
+  Qed.
+
+  Lemma get_polarity_rec_vars_res : forall v v' c b l,
+      Elim.get_polarity_rec v' c = Some (b, l) ->
+      is_var_of_clause v l -> is_var_of_clause v c.
+  Proof.
+    induction c.
+    - simpl. discriminate.
+    - simpl. intros.
+      destruct (get_pol v' a) eqn:POL.
+      inv H.
+      rewrite is_var_of_clause_cons. tauto.
+      destruct (Elim.get_polarity_rec v' c) eqn: P.
+      destruct p. inv H.
+      rewrite is_var_of_clause_cons in *.
+      intuition.
+      specialize (IHc _ _ eq_refl).
+      tauto.
+      discriminate.
+  Qed.
+
+
+ Lemma split_polarity_vars_spec : forall v' v cls lp ln lo,
+      Elim.split_polarity v' cls = (lp, ln, lo) ->
+      is_var_of_cnf v (lp++ln++lo) ->
+      is_var_of_cnf v cls /\ v <> v'.
+ Proof.
+   split.
+   - revert lp ln lo H H0.
+   induction cls.
+   + simpl. intros. inv H.
+     rewrite is_var_of_cnf_nil in H0.
+     tauto.
+   + intros.
+     simpl in H.
+     destruct (Elim.split_polarity v' cls) as ((lp',ln'),lo').
+     specialize (IHcls _ _ _ eq_refl).
+     destruct (Elim.normalise a) eqn:N.
+     apply normalise_vars with (p:= v) in N.
+     destruct (Elim.get_polarity_rec v' c) eqn:GP.
+     destruct p. inv H.
+     rewrite! is_var_of_cnf_app in H0.
+     rewrite is_var_of_cnf_cons.
+     specialize (get_polarity_rec_vars_res v _ _ _ _ GP).
+     rewrite! is_var_of_cnf_app in *.
+     destruct b; rewrite !is_var_of_cnf_cons in *.
+     tauto. tauto.
+     inv H.
+     rewrite is_var_of_cnf_cons.
+     rewrite! is_var_of_cnf_app in *.
+     rewrite is_var_of_cnf_cons in *.
+     tauto.
+     rewrite is_var_of_cnf_cons.
+     rewrite! is_var_of_cnf_app in *.
+     inv H.
+     tauto.
+   - apply split_polarity_vars in H.
+     rewrite! is_var_of_cnf_app in H0.
+     intuition congruence.
+ Qed.
+
+
+   
+  Lemma is_var_of_cnf_elim : forall v v' cls,
+      is_var_of_cnf v (Elim.elim v' cls) -> (is_var_of_cnf v cls /\ v <> v').
+  Proof.
+    unfold Elim.elim.
+    intros.
+    destruct (Elim.split_polarity v' cls) as ((lp,ln),lo) eqn:E.
+    apply split_polarity_vars_spec with (v:=v)    in E;auto.
+    rewrite is_var_of_cnf_app in H.
+    rewrite! is_var_of_cnf_app.
+    intuition.
+    apply is_var_of_cnf_resolve in H0.
+    rewrite! is_var_of_cnf_app in H0.
+    tauto.
+  Qed.
+
+  Lemma wf_cons : forall l cl,
+      wf (l :: cl) -> if pol l then Forall (fun l => pol l = true) cl else wf cl.
+  Proof.
+    intros.
+    unfold wf in H.
+    destruct H as (l1 & l2 & EQ); subst.
+    destruct l1. simpl in EQ.
+    destruct l; simpl;auto.
+    destruct l2. inv EQ.
+    inv EQ.
+    rewrite Forall_map.
+    rewrite Forall_forall.
+    reflexivity.
+    destruct l2 ; discriminate.
+    inv EQ.
+    simpl.
+    exists l1,l2;auto.
+  Qed.
+
+  Lemma wf_tl : forall l cl,
+      wf (l :: cl) -> wf cl.
+  Proof.
+    unfold wf. intros.
+    destruct H as (l1 & l2 & EQ); subst.
+    destruct l1. simpl in EQ. destruct l2; try discriminate.
+    inv EQ. exists nil,l2. reflexivity.
+    inv EQ.
+    exists l1,l2. reflexivity.
+  Qed.
+
+  Lemma get_polarity_rec_all_pos : forall p cl,
+      Forall (fun l : t => pol l = true) cl ->
+      forall b cl',
+      Elim.get_polarity_rec p cl = Some (b, cl') ->
+      b = true /\ Forall (fun l : t => pol l = true) cl'.
+  Proof.
+    intros p cl ALL.
+    induction ALL.
+    - simpl. discriminate.
+    - intros.
+      simpl in H0.
+      destruct (get_pol p x) eqn:GP.
+      + inv H0. apply get_pol_inv in GP.
+      subst.
+      destruct b; try discriminate.
+      tauto.
+      + destruct (Elim.get_polarity_rec p l) eqn:GP'; try discriminate.
+        destruct p0. inv H0.
+        specialize (IHALL _ _ eq_refl).
+        intuition.
+  Qed.
+
+
+
+  
+ Lemma get_polarity_ispec :
+  forall env p cl
+    (WF : wf cl),
+    match Elim.get_polarity_rec p cl with
+         | None => ~ is_var_of_clause  p  cl
+         | Some (b,cl') =>
+             eval_clause env cl <-> eval_clause env (cons_lit (Lit.make b p) cl')
+         end.
+Proof.
+  induction cl.
+  - simpl. rewrite is_var_of_clause_nil. tauto.
+  - intros.
+    simpl.
+    destruct (Lit.get_pol p a) eqn:GP.
+    apply Lit.get_pol_inv in GP.
+    subst.
+    +
+      apply wf_cons in WF.
+      destruct (pol (make b p)) eqn:POL.
+      rewrite eval_clause_cons_lit_POS by auto.
+      tauto.
+      rewrite eval_clause_cons_lit_NEG by auto.
+      tauto.
+    + destruct (Elim.get_polarity_rec p cl) eqn:GP'.
+      destruct p0 as (b,cl').
+      simpl.
+      assert (WFT := wf_tl a cl WF).
+      apply wf_cons in WF.
+      destruct (pol a) eqn:PA.
+      * simpl.
+        rewrite IHcl by auto.
+        apply get_polarity_rec_all_pos in GP';auto.
+        destruct GP';subst.
+        rewrite <- !eval_clause_cons_lit_POS; auto.
+        simpl. destruct a ; try discriminate.
+        unfold eval_lit ; simpl. tauto.
+      * simpl.
+        rewrite IHcl by auto.
+        destruct b; simpl.
+        unfold make. tauto.
+        rewrite! cons_lit_POS_false by reflexivity.
+        simpl.
+        destruct a; try discriminate. unfold eval_lit.
+        simpl. tauto.
+      * apply wf_tl in WF.
+        apply get_pol_None in GP.
+        rewrite is_var_of_clause_cons.
+        intuition congruence.
+Qed.
+
+
+Lemma sublist_normalise :
+  forall  cl cl',
+          Elim.normalise cl = Some cl' ->
+          sublist cl' cl.
+Proof.
+  induction cl.
+  - simpl. intros. inv H; auto. constructor.
+  - simpl; intros.
+    destruct (Elim.normalise cl) eqn:N.
+    + simpl in *.
+    intros.
+    destruct (Elim.get_polarity_rec (var a) c) eqn:POL.
+    * destruct p.
+      destruct (eq_dec (make (negb b) (var a)) a); try discriminate.
+      inv H.
+      specialize (IHcl _ eq_refl).
+      apply SUB_CONS;auto.
+    * inv H.
+      apply SUB_CONS2; auto.
+    + discriminate.
+Qed.
+
+Lemma wf_normalise :
+  forall  cl cl',
+    wf cl ->
+    Elim.normalise cl = Some cl' ->
+    wf cl'.
+Proof.
+  intros.
+  apply sublist_normalise in H0.
+  eapply wf_sublist; eauto.
+Qed.
+
+(*Lemma cons_lit_neg : forall env l a,
+    eval_lit env a (eval_clause env (cons_lit (neg a) l)).
+Proof.
+  induction l.
+  - simpl. destruct a; unfold eval_lit; simpl. tauto.
+*)
+
+Lemma wf_cons_sublist : forall a cl c,
+    wf (a :: cl) ->
+    sublist c cl ->
+    wf (a :: c).
+Proof.
+  intros.
+  apply wf_cons in H.
+  destruct (pol a) eqn:PA.
+  - unfold wf.
+  exists nil, (map var (a::c)).
+  simpl.
+  f_equal.
+  destruct a; try discriminate;auto.
+  rewrite map_map.
+  apply sublist_forall with (P:= Lit.isPOS) in H0; auto.
+  induction H0 ; simpl. reflexivity.
+  destruct x ; try discriminate.
+  f_equal. auto.
+  - apply wf_sublist in H0;auto.
+    unfold wf in H0.
+    destruct H0 as (l1&l2& EQ).
+    subst.
+    destruct a; try discriminate.
+    exists (p::l1),l2.
+    reflexivity.
+Qed.
+
+Lemma get_polarity_rec_sublist : forall p cl b cl',
+    Elim.get_polarity_rec p cl = Some(b,cl') ->
+    sublist cl' cl /\ In (make b p) cl.
+Proof.
+  induction cl.
+  - simpl. discriminate.
+  - simpl. intros.
+    destruct (get_pol p a) eqn:GP.
+    inv H.
+    apply get_pol_inv in GP.
+    split ; intuition.
+    constructor.
+    apply sublist_refl.
+    destruct (Elim.get_polarity_rec p cl) eqn: GP'.
+    destruct p0.
+    inv H. apply get_pol_None in GP.
+    specialize (IHcl _ _ eq_refl).
+    intuition.
+    apply SUB_CONS2. auto.
+    discriminate.
+Qed.
+
+Lemma eval_clause_cons_lit_tauto : forall (env: positive -> Prop) p l,
+    env p -> eval_clause env (cons_lit (POS p) l).
+Proof.
+  induction l;simpl.
+  - unfold eval_lit. simpl. tauto.
+  - rewrite orb_false_r.
+    destruct (pol a). simpl. unfold eval_lit. simpl.
+    destruct (pol a). tauto.
+    tauto.  simpl.
+    intros.
+    destruct a; unfold eval_lit; simpl.
+    tauto. tauto.
+Qed.
+
+Lemma cons_lit_twice : forall env a l,
+  eval_lit env a (eval_clause env (cons_lit a l)) <-> eval_clause env (cons_lit a l).
+Proof.
+  induction l; simpl.
+  -  unfold eval_lit. destruct a; simpl. tauto.
+     tauto.
+  - destruct a0; simpl.
+    unfold eval_lit.
+    destruct a; simpl.
+    tauto.
+    tauto.
+    destruct (pol a) eqn:A; simpl.
+    unfold eval_lit. rewrite A. simpl.
+    destruct a; try discriminate.
+    simpl.
+    unfold eval_lit in IHl. simpl in *.
+    tauto.
+    unfold eval_lit.
+    simpl. rewrite A.
+    tauto.
+Qed.
+
+Lemma eval_normalise :
+  forall env cl
+         (WF : wf cl),
+    eval_clause env cl <-> eval_option (eval_clause env) (Elim.normalise cl).
+Proof.
+  intros.
+  induction cl.
+  - simpl. tauto.
+  - simpl.
+    destruct (Elim.normalise cl) eqn:N.
+    +
+      assert (SL : sublist c cl).
+      {
+        apply sublist_normalise in N; auto.
+      }
+      simpl in *. intros.
+      assert (WFTL := wf_tl _ _ WF).
+      specialize (IHcl WFTL).
+      apply wf_normalise in N; auto.
+      generalize (get_polarity_ispec env (var a) c N).
+      destruct (Elim.get_polarity_rec (var a) c) eqn:POL.
+      * destruct p.
+        destruct (eq_dec (make (negb b) (var a)) a); simpl;auto.
+        intros.
+        split ; auto.
+        intros.
+        rewrite IHcl.
+        rewrite H.
+        assert (make b (var a) = Lit.neg a).
+        { rewrite <- e. destruct b; simpl;auto.}
+        rewrite H1.
+        assert (POL':= POL).
+        apply get_polarity_rec_sublist in POL.
+        destruct POL as (POL & IN).
+        rewrite H1 in IN.
+        assert (WFC : wf (a::c)).
+        {           eapply wf_cons_sublist;eauto. }
+        assert (WFL : wf (a::l)).
+        {
+          eapply wf_cons_sublist;eauto.
+        }
+        apply wf_cons in WFC.
+        destruct (pol a) eqn:PA.
+        destruct a ; try discriminate.
+        rewrite Forall_forall in WFC.
+        apply WFC in IN. discriminate.
+        destruct a; try discriminate.
+        simpl. unfold eval_lit ; simpl.
+        apply eval_clause_cons_lit_tauto.
+        intros.
+        apply make_var in n.
+        rewrite negb_involutive in n.
+        rewrite n in *.
+        rewrite IHcl.
+        rewrite H.
+        apply cons_lit_twice.
+      * simpl.
+        intros.
+        rewrite IHcl.
+        tauto.
+    + simpl in *.
+      apply wf_tl in WF.
+      rewrite IHcl by auto.
+      unfold eval_lit. destruct (pol a).
+      tauto.
+      tauto.
+Qed.
+
+Lemma split_polarity_ieval:
+  forall (env : positive -> Prop) (p : positive) (l lp ln lo : cnf)
+           (WF : Forall wf l)
+    ,
+  Elim.split_polarity p l = (lp, ln, lo) ->
+  eval_cnf env l ->
+    (eval_cnf env lo /\ eval_cnf env (map (cons_lit (POS p)) lp) /\
+       eval_cnf env (map (cons_lit (NEG p)) ln)).
+  Proof.
+  induction l.
+  - simpl; intros.
+    inv H.
+    simpl. tauto.
+  -  intros.
+     simpl in H.
+     simpl.
+     destruct (Elim.split_polarity p l) as [[lp' ln'] lo'] eqn:E.
+     inv WF.
+     specialize (IHl lp' ln' lo' H4 eq_refl).
+     simpl in H0.
+     rewrite eval_normalise in H0;auto.
+     destruct (Elim.normalise a) eqn:N; simpl.
+     +
+       apply wf_normalise in N; auto.
+       generalize (get_polarity_ispec env p c N).
+       destruct (Elim.get_polarity_rec p c).
+       *
+       destruct p0 as [b cl'].
+       inv H.
+       intros.
+       simpl in H0.
+       destruct b;
+       simpl;
+       intuition.
+       * inv H.
+         simpl in *.
+         intuition.
+     +  inv H. tauto.
+  Qed.
+
+  Lemma wf_split_polarity:
+    forall  (p : positive) (l lp ln lo : cnf)
+           (WF : Forall wf l)
+    ,
+      Elim.split_polarity p l = (lp, ln, lo) ->
+      Forall wf lp /\ Forall wf ln /\ Forall wf lo.
+  Proof.
+    induction l.
+    - simpl; intros.
+      inv H.
+      simpl. tauto.
+    -  intros.
+       simpl in H.
+       destruct (Elim.split_polarity p l) as [[lp' ln'] lo'] eqn:E.
+       inv WF.
+       specialize (IHl lp' ln' lo' H3 eq_refl).
+       destruct (Elim.normalise a) eqn:N; simpl.
+       +
+         apply wf_normalise in N; auto.
+         destruct (Elim.get_polarity_rec p c) eqn:GP.
+         *
+           destruct p0 as [b cl'].
+           apply get_polarity_rec_sublist in GP.
+           destruct GP.
+           apply wf_sublist in H0;auto.
+           destruct b; inv H; intuition.
+         * inv H. intuition.
+       + inv H;intuition.
+Qed.
+
+Lemma split_clause_wf : forall l1 l2,
+    Elim.split_clause (map NEG l1 ++ map POS l2) = (map NEG l1 , map POS l2).
+Proof.
+  induction l1;simpl.
+  -  destruct l2 ; reflexivity.
+  -  intros. rewrite IHl1. reflexivity.
+Qed.
+
+Lemma wf_merge_clause :
+  forall c1 c2,
+    wf c1 -> wf c2 ->
+    wf (Elim.merge_clause c1 c2).
+Proof.
+  intros.
+  unfold wf in *.
+  destruct H as (l1 & l2 & EQ).
+  destruct H0 as (l1' & l2' & EQ').
+  subst.
+  exists (l1 ++ l1') ,(l2 ++ l2').
+  unfold Elim.merge_clause.
+  rewrite! split_clause_wf.
+  rewrite! map_app.
+  rewrite <- !app_assoc.
+  reflexivity.
+Qed.
+
+Lemma cons_lit_POS_wf : forall v l1 l2,
+    (cons_lit (POS v) (map NEG l1 ++ map POS l2)) =
+      map NEG l1 ++ (map POS (v::l2)).
+Proof.
+  induction l1;simpl.
+  - destruct l2 ; reflexivity.
+  - intros.
+    f_equal.
+    rewrite IHl1. reflexivity.
+Qed.
+
+Lemma cons_lit_NEG_wf : forall v l1 l2,
+    (cons_lit (NEG v) (map NEG l1 ++ map POS l2)) =
+      map NEG (v::l1) ++ (map POS l2).
+Proof.
+  destruct l1;simpl;auto.
+  destruct l2;simpl;auto.
+Qed.
+
+Definition eval_or {A: Type} (F : A -> Prop) (l : list A) :=
+  List.fold_right (fun e acc => F e \/ acc) False l.
+
+Definition eval_and {A: Type} (F : A -> Prop) (l : list A) :=
+  List.fold_right (fun e acc => F e /\ acc) True l.
+
+Lemma eval_or_app : forall {A: Type} (F: A-> Prop) l1 l2,
+    eval_or F (l1++l2) <-> (eval_or F l1 \/ eval_or F l2).
+Proof.
+  induction l1;simpl.
+  - tauto.
+  - intros. rewrite IHl1. tauto.
+Qed.
+
+
+Lemma eval_clause_or : forall env l,
+    eval_clause env (map POS l) <-> eval_or env l.
+Proof.
+  induction l;simpl.
+  - tauto.
+  - rewrite IHl. unfold eval_lit. simpl. tauto.
+Qed.
+
+Lemma eval_clause_wf : forall env l1 l2,
+    eval_clause env (map NEG l1 ++ l2) <-> (eval_and env l1 -> eval_clause env l2).
+Proof.
+  induction l1.
+  - simpl.
+    intros. tauto.
+  - simpl. intros.
+    rewrite IHl1.
+    unfold eval_lit. simpl. tauto.
+Qed.
+
+Lemma merge_clause_correct : forall env v cl cl',
+    wf cl -> wf cl' ->
+    eval_clause env (cons_lit (POS v) cl) ->
+    eval_clause env (cons_lit (NEG v) cl') ->
+    eval_clause env (Elim.merge_clause cl cl').
+Proof.
+  intros.
+  unfold wf in *.
+  destruct H as (l1 & l2 & EQ).
+  destruct H0 as (l1' & l2' & EQ').
+  subst.
+  unfold Elim.merge_clause.
+  rewrite! split_clause_wf.
+  rewrite cons_lit_NEG_wf in H2.
+  rewrite cons_lit_POS_wf in H1.
+  simpl in H2.
+  repeat rewrite eval_clause_wf  in *.
+  unfold eval_lit in H2. simpl in H2.
+  intros.
+  rewrite <- map_app.
+  rewrite eval_clause_or.
+  rewrite eval_or_app.
+  rewrite eval_clause_or in *.
+  simpl in H1. unfold eval_lit in H1. simpl in H1.
+  tauto.
+Qed.
+
+
+Lemma elim_correct : forall env v cls
+                              (WF: Forall wf cls),
+      eval_cnf env cls ->
+      eval_cnf env (Elim.elim v cls).
+  Proof.
+    unfold Elim.elim.
+    intros.
+    destruct (Elim.split_polarity v cls) as ((lp,ln),lo) eqn:SP.
+    assert (SP':=SP).
+    apply split_polarity_ieval with (env:=env) in SP;auto.
+    destruct SP as (SP1 & SP2 & SP3).
+    apply wf_split_polarity in SP'; auto.
+    rewrite eval_cnf_app.
+    split ;auto.
+    destruct SP' as [WF1 [WF2 WF3]].
+    revert ln SP3 WF2.
+    induction lp.
+    - simpl. auto.
+    - simpl.
+      intros.
+      simpl in SP2.
+      rewrite eval_cnf_app.
+      intuition.
+      clear H2.
+      clear H1.
+      induction ln.
+      + simpl. auto.
+      + simpl.
+        simpl in SP3.
+        assert (wf (Elim.merge_clause a a0)).
+        {
+          inv WF1. inv WF2.
+          apply wf_merge_clause;auto.
+        }
+        generalize (eval_normalise env _ H1).
+        destruct (Elim.normalise (Elim.merge_clause a a0)).
+        simpl.
+        intros. split.
+        rewrite <- H2.
+        eapply merge_clause_correct;eauto.
+        inv WF1;auto.
+        inv WF2;auto.
+        tauto.
+        apply IHln.
+        tauto.
+        inv WF2;auto.
+        simpl.
+        intros. apply IHln;auto.
+        tauto. inv WF2;auto.
+      +  apply H2;auto.
+         inv WF1;auto.
+Qed.
+
+  Lemma wf_resolve_all : forall lp ln
+                                (WF1 : Forall wf lp)
+                                (WF2 : Forall wf ln)
+    ,
+
+    Forall wf (Elim.resolve_all lp ln).
+Proof.
+  induction lp.
+  - simpl. constructor.
+  - simpl. intros.
+    rewrite Forall_app. split; auto.
+    assert (Forall wf (map (Elim.merge_clause a) ln)).
+    inv WF1.
+    induction ln.
+    constructor.
+    simpl.
+    constructor.
+    apply wf_merge_clause;auto. inv WF2;auto.
+    apply IHln. inv WF2;auto.
+    induction  ((map (Elim.merge_clause a) ln)).
+    + simpl. constructor.
+    + simpl.  inv H.
+      destruct (Elim.normalise a0) eqn:N.
+      constructor.
+      eapply wf_normalise;eauto.
+      apply IHl;auto. apply IHl;auto.
+    + apply IHlp;auto.
+      inv WF1;auto.
+Qed.
+
+
+Lemma wf_elim : forall x cls,
+    Forall wf cls ->
+    Forall wf (Elim.elim x cls).
+Proof.
+  unfold Elim.elim.
+  intros.
+  destruct (Elim.split_polarity x cls) as ((lp,ln),lo) eqn:SP.
+  apply wf_split_polarity  in SP; auto.
+  rewrite Forall_app.
+  split ; try tauto.
+  apply wf_resolve_all;tauto.
+Qed.
+
+
+  Lemma eval_clause_classic :
+  forall cls i (WF: Forall wf cls),
+    (forall env, beval_cnf env cls = true -> boeval env i = true) ->
+    (forall env, eval_cnf env cls  -> oeval env i).
+Proof.
+  intros.
+  set (L := vars_of_cnf cls).
+  assert (ND := NoDup_nodup positive_eq_dec L).
+  apply has_cardinal_no_dup in ND.
+  assert (Lspec :
+           forall v : positive, is_var_of_cnf v cls -> In v (nodup Pos.eq_dec L)).
+  {
+    intros.
+    rewrite nodup_In.
+    apply vars_of_cnf_ok; auto.
+  }
+  revert ND H0.
+  generalize (length (nodup Pos.eq_dec L)) as n.
+  intro.
+  unfold L in *.
+  clear L. revert Lspec.
+  generalize ((nodup Pos.eq_dec (vars_of_cnf cls))) as vars.
+  revert cls WF H.
+  induction n.
+  - intros.
+    inv ND.
+    simpl in Lspec.
+    assert (LspecFalse := is_var_of_cnf_False cls Lspec).
+    destruct cls.
+    + simpl in H0.
+      specialize (H (fun x => false) eq_refl).
+      destruct i; simpl in *;discriminate.
+    + simpl in H0.
+      destruct H0.
+      assert (c = nil).
+      apply LspecFalse. simpl; tauto.
+      subst.
+      simpl in H0. tauto.
+  - intros.
+    inv ND.
+    destruct (match_option_dec x i).
+    + destruct i ; simpl in *; try tauto.
+      subst.
+      destruct l.
+      * assert (IN : forall v, is_var_of_cnf v cls -> p = v).
+      {
+        intros.
+        apply Lspec in H1. simpl in H1.
+        tauto.
+      }
+      eapply beval_clauses_one_var in H.
+      destruct H as (cl & INC & ALLP).
+      eapply eval_clauses_all_pos ; eauto.
+      intros.
+      apply Lspec in H1. simpl in H1. tauto.
+      *
+        set (E := Elim.elim  p0 cls).
+        eapply IHn with (cls:= E) (vars:= (p::l)); auto.
+        apply wf_elim;auto.
+        {
+          rewrite neg_concl with (l:= Some p) in H.
+          rewrite neg_concl with (l:= Some p).
+          intros.
+          apply elim_complete with (env:=env0) (p:= p0) in H.
+          tauto.
+          rewrite elim_no_vars.
+          auto.
+          simpl. rewrite is_var_of_cnf_cons.
+          rewrite is_var_of_cnf_nil.
+          rewrite is_var_of_clause_cons.
+          rewrite is_var_of_clause_nil.
+          simpl. simpl in H4. intuition congruence.
+        }
+        {
+          intros.
+          apply is_var_of_cnf_elim in H1.
+          destruct H1.
+          apply Lspec in H1.
+          simpl in *. intuition congruence.
+        }
+        { inv H2. constructor;auto. simpl in H4. tauto. }
+        { apply elim_correct; auto. }
+    +   set (E := Elim.elim x cls).
+        eapply IHn with (cls:= E) (vars:= l); auto.
+        apply wf_elim;auto.
+        {
+          intros.
+          rewrite neg_concl with (l:= i) in H.
+          destruct (boeval env0 i) eqn:EI;auto.
+          exfalso.
+          apply elim_complete with (env:=env0) (p:= x) in H; auto.
+          rewrite elim_no_vars.
+          rewrite beval_cnf_app.
+          unfold E in H3. rewrite H3.
+          rewrite eval_clause_of_opt.
+          rewrite EI. reflexivity.
+          destruct i; simpl in *.
+          rewrite is_var_of_cnf_cons.
+          rewrite is_var_of_clause_cons.
+          rewrite is_var_of_cnf_nil.
+          rewrite is_var_of_clause_nil.
+          simpl.  intuition congruence.
+          rewrite is_var_of_cnf_nil. tauto.
+        }
+        {
+          intros.
+          apply is_var_of_cnf_elim in H3.
+          destruct H3.
+          apply Lspec in H3.
+          simpl in *. intuition congruence.
+        }
+        { apply elim_correct; auto.
+        }
+Qed.
