theories/Lib.v
@@ -1,0 +1,111 @@
+(* Copyright 2023 Frédéric Besson <frederic.besson@inria.fr> *)
+Require Import Bool ZifyBool ZArith ZifyUint63 Uint63 Lia.
+
+(* Some basic tactics and results *)
+
+Ltac inv H := inversion H ; try subst ; clear H.
+Ltac split_and :=
+  repeat
+    match goal with
+    | |- ?A /\ ?B => split ; split_and
+    end.
+
+Lemma and_first : forall A B : Prop,
+    A -> (A -> B) -> A /\ B.
+Proof.  tauto. Qed.
+
+Ltac split_and_first :=
+  match goal with
+  | |- _ /\ _ => apply and_first ; [| intro ; split_and_first]
+  | |- _ => idtac
+  end.
+
+Ltac destruct_in_goal eqn :=
+  match goal with
+  | |- context[match ?X with
+               | _ => _
+               end] => destruct X eqn: eqn
+  end.
+
+Ltac destruct_in_hyp H eqn :=
+  match type of H with
+  | context[match ?X with
+                | _ => _
+            end]  => destruct X eqn: eqn
+  end.
+
+(** Comparison of uint63 *)
+
+Lemma compare_refl : forall i, (i ?= i)%uint63 = Eq.
+Proof.
+  intros.
+  rewrite compare_def_spec.
+  unfold compare_def.
+  replace (i <? i)%uint63 with false by lia.
+  replace (i =? i)%uint63 with true by lia.
+  reflexivity.
+Qed.
+
+Lemma compare_Eq : forall x y, (x ?= y)%uint63 = Eq <-> (x =? y = true)%uint63.
+Proof.
+  intros.
+  rewrite compare_def_spec.
+  unfold compare_def.
+  destruct (x <?y)%uint63 eqn:LT; try congruence.
+  intuition (congruence || lia).
+  destruct (x =?y)%uint63 ;   intuition (congruence || lia).
+Qed.
+
+Lemma compare_Lt : forall x y, (x ?= y)%uint63 = Lt <-> (x <? y = true)%uint63.
+Proof.
+  intros.
+  rewrite compare_def_spec.
+  unfold compare_def.
+  destruct (x <?y)%uint63 eqn:LT; try congruence.
+  intuition (congruence || lia).
+  destruct (x =?y)%uint63 ;   intuition (congruence || lia).
+Qed.
+
+Lemma compare_Gt : forall x y, (x ?= y)%uint63 = Gt <-> (y <? x = true)%uint63.
+Proof.
+  intros.
+  rewrite compare_def_spec.
+  unfold compare_def.
+  destruct (x <?y)%uint63 eqn:LT; try congruence.
+  intuition (congruence || lia).
+  destruct (x =?y)%uint63 eqn:EQ;   intuition (congruence || lia).
+Qed.
+
+Ltac elim_compare :=
+  match goal with
+  | H : (?X ?= ?Y)%uint63 = Eq |- _ => rewrite compare_Eq in H
+  | H : (?X ?= ?Y)%uint63 = Lt |- _ => rewrite compare_Lt in H
+  | H : (?X ?= ?Y)%uint63 = Gt |- _ => rewrite compare_Gt in H
+  | |-  (?X ?= ?Y)%uint63 = Eq  => rewrite compare_Eq
+  | |-  (?X ?= ?Y)%uint63 = Lt  => rewrite compare_Lt
+  | |-  (?X ?= ?Y)%uint63 = Gt  => rewrite compare_Gt
+  end.
+
+Lemma lift_if : forall (P: bool -> Prop), forall x, (x =  true -> P true) /\ (x = false -> P false)  -> P x.
+Proof.
+  destruct x ; tauto.
+Qed.
+
+Ltac lift_if :=
+  match goal with
+  | |- context[if ?x then _ else _ ] => pattern x ; apply lift_if
+  end.
+
+Ltac elim_match_comparison :=
+  match goal with
+  | |- context[match ?X with
+       | Eq => _
+       | Lt => _
+       | Gt => _
+       end] => let F := fresh in destruct X eqn:F
+  | H: context[match ?X with
+       | Eq => _
+       | Lt => _
+       | Gt => _
+       end] |- _ => let F := fresh in destruct X eqn:F
+  end.
